basis/fsFFIScript.sml
@@ -7,7 +7,11 @@ val _ = new_theory"fsFFI"
 
 val _ = option_monadsyntax.temp_add_option_monadsyntax();
 
-val _ = Datatype` inode = IOStream mlstring | File mlstring`
+
+(* Logical model of filesystem and I/O streams *)
+
+(* regular files and unnamed streams *)
+val _ = Datatype` inode = UStream mlstring | File mlstring`
 
 val _ = overload_on("isFile",``λinode. ∃fnm. inode = File fnm``);
 
@@ -25,8 +29,9 @@ val _ = Datatype` mode = ReadMode | WriteMode`;
 
 val _ = Datatype`
   IO_fs = <| files : (inode # char list) list ;
+             inode_tbl : (mlstring # mlstring) list;
              infds : (num # (inode # mode # num)) list;
-             numchars : num llist ;
+             numchars : num llist;
              maxFD : num
            |>`
 
@@ -56,8 +61,9 @@ val openFile_def = Define`
      in
        do
           assert (fd <= fsys.maxFD) ;
-          ALOOKUP fsys.files (File fnm);
-          return (fd, fsys with infds := (nextFD fsys, (File fnm, md, pos)) :: fsys.infds)
+          iname <- ALOOKUP fsys.inode_tbl fnm;
+          ALOOKUP fsys.files (File iname);
+          return (fd, fsys with infds := (nextFD fsys, (File iname, md, pos)) :: fsys.infds)
        od
 `;
 
@@ -74,9 +80,10 @@ val openFile_truncate_def = Define`
     let fd = nextFD fsys in
       do
         assert (fd <= fsys.maxFD) ;
-        ALOOKUP fsys.files (File fnm);
-        return (fd, (fsys with infds := (nextFD fsys, (File fnm, md, 0)) :: fsys.infds)
-                          with files updated_by (ALIST_FUPDKEY (File fnm) (\x."")))
+        iname <- ALOOKUP fsys.inode_tbl fnm;
+        ALOOKUP fsys.files (File iname);
+        return (fd, (fsys with infds := (nextFD fsys, (File iname, md, 0)) :: fsys.infds)
+                          with files updated_by (ALIST_FUPDKEY (File iname) (\x."")))
       od `;
 
 (* checks if a descriptor index is in infds *)
@@ -278,7 +285,7 @@ val ffi_close_def = Define`
 (* Packaging up the model as an ffi_part *)
 
 val encode_inode_def = Define`
-  (encode_inode (IOStream s) = Cons (Num 0) ((Str o explode) s)) /\
+  (encode_inode (UStream s) = Cons (Num 0) ((Str o explode) s)) /\
   encode_inode (File s) = Cons (Num 1) ((Str o explode) s)`;
 
 val encode_files_def = Define`
@@ -292,14 +299,19 @@ val encode_fds_def = Define`
   encode_fds fds =
      encode_list (encode_pair Num (encode_pair encode_inode (encode_pair encode_mode Num))) fds`;
 
+val encode_inode_tbl_def = Define`
+  encode_inode_tbl fs = encode_list (encode_pair (Str o explode) (Str o explode)) fs`;
+
 val encode_def = zDefine`
   encode fs = Cons
-               (cfFFIType$Cons
+               (Cons
                  (cfFFIType$Cons
-                   (encode_files fs.files)
-                   (encode_fds fs.infds))
-                 (Stream fs.numchars))
-                (Num fs.maxFD)`
+                  (cfFFIType$Cons
+                    (encode_files fs.files)
+                    (encode_fds fs.infds))
+                  (Stream fs.numchars))
+                 (encode_inode_tbl fs.inode_tbl))
+               (Num fs.maxFD)`
 
 Theorem encode_inode_11[simp]
   `!x y. encode_inode x = encode_inode y <=> x = y`
@@ -320,6 +332,12 @@ Theorem encode_fds_11[simp]
   (rw [] \\ eq_tac \\ rw [encode_fds_def]
   \\ drule encode_list_11
   \\ fs [encode_pair_def,FORALL_PROD,encode_inode_def]);
+
+Theorem encode_inode_tbl_11[simp]
+  `!xs ys. encode_inode_tbl xs = encode_inode_tbl ys <=> xs = ys`
+ (rw [] \\ eq_tac \\ rw [encode_inode_tbl_def]
+  \\ drule encode_list_11
+  \\ fs [encode_pair_def,FORALL_PROD]);
 
 Theorem encode_11[simp]
   `!x y. encode x = encode y <=> x = y`
