tutorial/splitwordsScript.sml
@@ -32,14 +32,15 @@ Theorem splitwords_concat_space
 
 Theorem splitwords_all_lines
   `FLAT (MAP splitwords (all_lines fs fname)) =
-   splitwords (implode (THE (ALOOKUP fs.files fname)))`
-  (`isSpace #"\n"` by EVAL_TAC \\
+   splitwords (implode (THE (ALOOKUP fs.files
+                         (File (THE(ALOOKUP fs.file_inode fname))))))`
+  `isSpace #"\n"` by EVAL_TAC \\
   rw[all_lines_def,lines_of_def,MAP_MAP_o,o_DEF,
      GSYM mlstringTheory.str_def,splitwords_concat_space] \\
   rw[splitwords_def,mlstringTheory.TOKENS_eq_tokens_sym] \\
   srw_tac[ETA_ss][GSYM o_DEF,GSYM MAP_MAP_o] \\
   simp[GSYM MAP_FLAT] \\ AP_TERM_TAC \\
-  qspec_tac(`THE (ALOOKUP fs.files fname)`,`ls`) \\
+  qmatch_goalsub_rename_tac `splitlines ls` \\
   rw[splitlines_def]
   >- (
     qmatch_asmsub_abbrev_tac`NULL (LAST l)` \\
